Issue with NotAVar exception

tele.v
@@ -46,23 +46,23 @@ Module V2.
       | [? A] (M A):Type =>
           ret (MTele_ConstT A m)
       | [? T1 T2] T1 -> T2 =>
-          M.print "implication";;
+          M.print "BRANCH implication";;
           t1 <- f T1;
           t2 <- f T2;
           ret (t1 -> t2)
       | [? (V : forall X : Type, Type)] (forall X : Type, V X) =>
-          M.print "forall1";;
+          M.print "BRANCH forall1";;
           \nu_f for A as X : MTele_Ty m,
               v <- f (V (@repl m X));
               abs_prod_type X v
       | [? (V : forall X : Type, Prop)] (forall X : Type, V X):Type =>
-          M.print "forall1prop";;
+          M.print "BRANCH forall1_prop";;
           \nu_f for A as X : MTele_Ty m,
               let x := reduce (RedOneStep [rl:RedBeta]) (V (@repl m X)) in
               v <- f (x);
               abs_prod_type X v
       | [? T (V : forall x : T, Type)] (forall t : T, V t) =>
-          M.print "forall2";;
+          M.print "BRANCH forall2";;
           \nu_f for A as t : T,
               v1 <- f (V t);
               abs_prod_type t v1
@@ -76,9 +76,120 @@ Module V2.
 
   Goal MTele -> Type.
   intros m.
-  mrun (lift' (@ret) m).
+  mrun (lift' (@bind) m).
   Show Proof. Abort.
 
 End V2.
 
-@bind A (B c) ma (fun a => f a c)
+Module V3.
+  
+  Local Notation MFA T := (MTele_val (MTele_C SType SProp M T)).
+
+  Polymorphic Definition repl {m : MTele} {s : Sort} (A : MTele_Sort s m) := MTele_val A.
+  
+  (* This would only be applied in negative parts *)
+  (* I pass a list [X; Y] and a type A and returns X Y sniped and
+     A with the new X and Y *)
+  (* Definition lift_neg (l : list Type) (A : Type) (m : MTele) : M Type := *)
+  (*     let r := (mfix1 f (A : Type) : M (MTele_Sort SType m) := *)
+  (*         mmatch A in Type as A' return M (MTele_Sort SType m) with *)
+  (*         | [? A B] A -> B => *)
+  (*             \nu A' : MTele_Ty m; *)
+                  
+  (*         end) in *)
+  (*     v <- r A; *)
+  (*     ret (MTele_val v). *)
+
+  Notation "'[withP' now_ty , now_val '=>' t ]" :=
+    (MTele_In (SProp) (fun now_ty now_val => t))
+  (at level 0, format "[withP now_ty , now_val => t ]").
+
+  (* Definition lift_conservative (A : Type) (m : MTele) : M (MTele_Ty m) := *)
+  (*     (mfix1 f (A : Type) : M (MTele_Ty m) := *)
+  (*         mmatch A in Type as A' return M (MTele_Ty m) with *)
+  (*         | [? A] @repl m A => *)
+  (*             ret (MTele_val A) *)
+  (*         | [? A] M (@repl m A) => *)
+  (*             _ *)
+  (*         end) A. *)
+
+  Polymorphic Definition lift_neg' (A : Type) (m : MTele) :
+  M (forall (now_ty : forall (s : Sort), MTele_Sort s m -> s)
+       (now_val : forall (s: Sort) (T : MTele_Sort s m), MTele_val T -> now_ty s T),
+        SType) :=
+      (mfix1 f (A : Type) :
+      M (forall (now_ty : forall (s : Sort), MTele_Sort s m -> s)
+           (now_val : forall (s: Sort) (T : MTele_Sort s m), MTele_val T -> now_ty s T),
+            SType) :=
+          mmatch A in Type as A' return
+          M (forall (now_ty : forall (s : Sort), MTele_Sort s m -> s)
+               (now_val : forall (s: Sort) (T : MTele_Sort s m), MTele_val T -> now_ty s T),
+                SType) with
+          | [? A] @repl m SType A =>
+              ret (fun fTy fVal => @fTy SType A)
+          (* | [? (A : MTele_Sort SType m)] (M (@repl m SType A)):Type => *)
+              (* ret (fun fTy fVal => *)
+                  (* let A' := @fTy SType A in *)
+                  (* (M A'):Type) *)
+          (* | [? A B] A -> B => *)
+          (*     A' <- f A; *)
+          (*     B' <- f B; *)
+          (*     ret (fun fTy fVal => *)
+          (*         let A' := fTy SType A' in *)
+          (*         let B' := fTy SType B' in *)
+          (*         (A' -> B')) *)
+          end) A.
+
+  Polymorphic Definition lift_neg (A : Type) (m : MTele) : M Type :=
+      F <- lift_neg' A m;
+      ret (MTele_val (@MTele_In _ m F)). 
+
+  (* Set Printing Universes. *)
+  Polymorphic Definition lift (A : Type) (m : MTele) : M Type :=
+    (mfix2 f (A : Type) (b : bool) : M Type :=
+      M.print_term A;;
+      mmatch A in Type as A' return M Type with
+      | [? m A] @repl m SType A =>
+          ret (MTele_val A)
+      | [? A] (M (@repl m SType A)):Type =>
+          ret ((MFA A):Type)
+      | [? A] (M A):Type =>
+          ret (MTele_ConstT A m)
+      | [? T1 T2] T1 -> T2 =>
+          M.print "implication";;
+          t1 <- lift_neg T1 m;
+          t2 <- f T2 true;
+          ret (t1 -> t2)
+      | [? (V : forall X : Type, Type)] (forall X : Type, V X) =>
+          M.print "forall1";;
+          \nu_f for A as X : MTele_Ty m,
+              v <- f (V (@repl m SType X)) true;
+              abs_prod_type X v
+      | [? (V : forall X : Type, Prop)] (forall X : Type, V X):Type =>
+          M.print "forall1prop";;
+          \nu_f for A as X : MTele_Ty m,
+              let x := reduce (RedOneStep [rl:RedBeta]) (V (@repl m SType X)) in
+              v <- f (x) true;
+              abs_prod_type X v
+      | [? T (V : forall x : T, Type)] (forall t : T, V t) =>
+          M.print "forall2";;
+          \nu_f for A as t : T,
+              v1 <- f (V t) true;
+              abs_prod_type t v1
+      | [? m V A] (V (@repl m SType A)) =>
+          M.failwith "Unused replace"
+      | _ =>
+          ret (A)
+      end) A true.
+
+  Polymorphic Definition lift' {A} (a : A) (m : MTele) := lift A m.
+
+  Polymorphic Definition bla : MTele -> Type.
+  intros m.
+  pose (t := ltac:(mrun (lift' (@ret) mBase))).
+  cbv iota zeta beta fix delta [MTele_In] in t.
+  mrun (lift' (@ret) m).
+Defined.
+  Show Proof. Abort.
+
+End V3.
